`EYield` before `kill_thread` to reduce the number of cases in heaplang adequacy.

src/heaplang/adequacy.v
@@ -1,4 +1,4 @@
-From iris.itree Require Import wpi ub.
+From iris.itree Require Import wpi ub itree.
 From iris.itree.threadpool Require Import trace.
 From iris Require Import invariants ghost_map.
 From iris.proofmode Require Import proofmode.
@@ -14,36 +14,36 @@ Lemma compile_Fork_value {R} e (k : val → itree heaplangE R) :
 Admitted.
 
 Lemma compile_Fork {R} e (k : val → itree heaplangE R) :
-  is_value e = false →
   (v ← compile_expr (Fork e) ; k v)%itree ≈ vis EFork (λ thread,
     match thread with
     | CurrentThread => k (LitV LitUnit)
     | NewThread =>
         v ← compile_expr e;
+        yield_if_not_val e;;
         kill_thread
     end
   )%itree.
 Proof.
-  intros Hval.
-  rewrite /compile_expr !rec_as_interp /= Hval interp_bind.
-  setoid_rewrite interp_trigger. simpl.
-  rewrite -bind_trigger bind_bind. f_equiv. intros [|].
-  - rewrite interp_ret bind_ret_l //.
-  - rewrite rec_as_interp interp_bind bind_bind. f_equiv. intros v.
-    rewrite /kill_thread. rewrite interp_vis /= bind_vis bind_vis.
-    apply eqit_VisF. intros [].
+  rewrite /compile_expr. simpl_itree. simpl_itree.
+  rewrite -bind_trigger. f_equiv. intros [|].
+  - by simpl_itree.
+  - simpl_itree. f_equiv. intros v. rewrite /kill_thread.
+      rewrite /yield_if_not_val. destruct (is_value _) eqn:Hval.
+      * rewrite /kill_thread. simpl_itree. rewrite -bind_trigger. f_equiv; first done.
+        intros [].
+      * rewrite /kill_thread. simpl_itree. f_equiv; first done.
+        intros []. rewrite -bind_trigger. f_equiv; first done. intros [].
 Qed.
 
 Lemma trace_base_Fork {R} tid (tp : list (itree heaplangE R)) tr e k :
-  is_value e = false →
   tp !! tid = Some (v ← compile_expr (Fork e) ; k v)%itree →
-  is_ctrace tr tid (<[tid := k (LitV LitUnit)]>tp ++ [(compile_expr e ;; kill_thread)%itree]) →
-  is_ctrace (CTFork (compile_expr e ;; kill_thread) tr) tid tp.
+  is_ctrace tr tid (<[tid := k (LitV LitUnit)]>tp ++ [(compile_expr e ;; yield_if_not_val e ;; kill_thread)%itree]) →
+  is_ctrace (CTFork (compile_expr e ;; yield_if_not_val e ;; kill_thread) tr) tid tp.
 Proof.
-  intros Hval Htp Htr. eapply is_ctrace_insert; first done; first apply compile_Fork; eauto.
+  intros Htp Htr. eapply is_ctrace_insert; first done; first apply compile_Fork; eauto.
   eexists. split. { rewrite list_lookup_insert //. by apply lookup_lt_is_Some_1. }
   constructor.
-  rewrite /compile_expr rec_as_interp //. rewrite list_insert_insert.
+  rewrite /compile_expr //. rewrite list_insert_insert.
   destruct Htr as (t'&Ht'&Htr).
   simpl in Ht'.
   rewrite lookup_app_l in Ht'; last rewrite insert_length -lookup_lt_is_Some //.
@@ -56,9 +56,7 @@ Lemma base_BinOp op v1 v2 v3 :
   compile_expr (BinOp op (Val v1) (Val v2)) ≈ Ret v3.
 Proof.
   intros Hop.
-  rewrite /compile_expr !rec_as_interp interp_bind interp_ret bind_ret_l /=
-    interp_bind interp_ret bind_ret_l interp_bind interp_ret bind_ret_l
-    interp_bind interp_ret bind_ret_l Hop interp_ret //.
+  rewrite /compile_expr. simpl_itree. rewrite Hop. by simpl_itree.
 Qed.
 
 Lemma base_Beta f_ x_ e v :
@@ -66,33 +64,15 @@ Lemma base_Beta f_ x_ e v :
   ≈ let e' := (subst' x_ v (subst' f_ (RecV f_ x_ e) e))
      in yield_if_not_val e' ;; compile_expr e'.
 Proof.
-  rewrite /compile_expr !rec_as_interp interp_bind interp_ret bind_ret_l /=
-    interp_bind interp_ret bind_ret_l interp_bind interp_ret bind_ret_l
-    interp_bind interp_ret bind_ret_l interp_bind /yield_if_not_val.
-  destruct (is_value _) eqn:Heq.
-  - rewrite interp_ret !bind_ret_l rec_as_interp.
-    setoid_rewrite interp_trigger. rewrite /= rec_as_interp //.
-  - setoid_rewrite interp_trigger. f_equiv; first done. by intros _.
+  rewrite /compile_expr. simpl_itree. rewrite /yield_if_not_val.
+  destruct (is_value _) eqn:Heq; by simpl_itree.
 Qed.
 
 Definition compile_tp (tp : list expr) : list (itree heaplangE ()) :=
-  map (λ e, compile_expr e ;; kill_thread)%itree (List.filter (λ e, negb (is_value e)) tp).
+  map (λ e, compile_expr e ;; yield_if_not_val e ;; kill_thread)%itree tp.
 
 Lemma compile_tp_app (tp tp' : list expr) :
   compile_tp (tp ++ tp') = compile_tp tp ++ compile_tp tp'.
-Admitted.
-
-Lemma compile_tp_cons (e : expr) (tp : list expr) :
-  compile_tp (e :: tp) = if is_value e then compile_tp tp else (compile_expr e ;; kill_thread)%itree :: compile_tp tp.
-Admitted.
-
-Lemma compile_tp_empty (tp : list expr) :
-  Forall is_value tp →
-  compile_tp tp = [].
-Admitted.
-Lemma compile_tp_empty_inv (tp : list expr) :
-  compile_tp tp = [] →
-  Forall is_value tp.
 Admitted.
 
 Lemma step_in_thread e1 σ1 κs e2 σ2 efs tr tid tid' tp (k : val → itree heaplangE ()) :
@@ -151,49 +131,15 @@ Proof.
   - admit.
   - admit.
   - admit.
-  - destruct (is_value e) eqn:Hval.
-    * rewrite /compile_tp in Htr. simpl in Htr. rewrite Hval /= in Htr.
-      exists (CTYield tid' tr).
-      split; first repeat constructor.
-      eapply is_ctrace_insert; first done; first apply compile_Fork_value; first done.
-      simpl.
-      eapply is_ctrace_yield.
-      { rewrite list_lookup_insert //. by apply lookup_lt_is_Some. }
-      rewrite list_insert_insert.
-      rewrite compile_expr_val !bind_ret_l in Htr.
-      by rewrite /= app_nil_r in Htr.
-    * exists (CTFork (compile_expr e ;; kill_thread) (CTYield tid' tr)).
-      split; first repeat constructor.
-      rewrite compile_expr_val !bind_ret_l in Htr.
-      eapply trace_base_Fork; first done; first apply Htp.
-      eapply is_ctrace_yield.
-      { rewrite lookup_app_l; last rewrite insert_length -lookup_lt_is_Some //.
-        rewrite list_lookup_insert //. by apply lookup_lt_is_Some. }
-      rewrite insert_app_l; last rewrite insert_length -lookup_lt_is_Some //.
-      rewrite list_insert_insert //. by rewrite /compile_tp /= Hval /= in Htr.
-Admitted.
-
-Lemma base_step_in_thread_completed e1 σ1 κs e2 σ2 efs tr tid tid' (tp : list (itree heaplangE ())) :
-  base_step e1 σ1 κs e2 σ2 efs →
-  is_value e2 →
-  is_ctrace tr tid' (delete tid tp ++ compile_tp efs) →
-  tp !! tid = Some (compile_expr e1 ;; kill_thread)%itree →
-  ∃ tr', is_postfix tr tr' ∧ is_ctrace tr' tid tp.
-Admitted.
-
-Lemma base_step_in_thread_not_completed e1 σ1 κs e2 σ2 efs tr tid tid' (tp : list (itree heaplangE ())) :
-  base_step e1 σ1 κs e2 σ2 efs →
-  ~is_value e2 →
-  is_ctrace tr tid' (<[tid:=(compile_expr e2 ;; kill_thread)%itree]>tp ++ compile_tp efs) →
-  tp !! tid = Some (compile_expr e1 ;; kill_thread)%itree →
-  ∃ tr', is_postfix tr tr' ∧ is_ctrace tr' tid tp.
-Admitted.
-
-Lemma base_step_in_thread_last_thread {R} e1 σ1 κs e2 σ2 efs tid :
-  base_step e1 σ1 κs e2 σ2 efs →
-  is_value e2 →
-  Forall is_value efs →
-  ∃ tr, is_ctrace (R := R) tr tid [(compile_expr e1 ;; kill_thread)%itree].
+  - exists (CTFork (compile_expr e ;; yield_if_not_val e ;; kill_thread) (CTYield tid' tr)).
+    split; first repeat constructor.
+    rewrite compile_expr_val !bind_ret_l in Htr.
+    eapply trace_base_Fork; first apply Htp.
+    eapply is_ctrace_yield.
+    { rewrite lookup_app_l; last rewrite insert_length -lookup_lt_is_Some //.
+      rewrite list_lookup_insert //. by apply lookup_lt_is_Some. }
+    rewrite insert_app_l; last rewrite insert_length -lookup_lt_is_Some //.
+    rewrite list_insert_insert //.
 Admitted.
 
 Lemma base_step_not_value e1 σ1 κs e2 σ2 tfs :
@@ -220,8 +166,7 @@ Lemma has_trace n tp σ tp' σ' κ :
 Proof.
   revert tp σ tp' σ' κ. induction n as [|n IH]; intros tp σ tp' σ' κ Hstep Hne.
   { exists CTCut, 0. apply is_ctrace_CTCut. rewrite map_length.
-    remember (length (List.filter (λ e : expr, negb (is_value e)) tp)).
-    rewrite /compile_tp map_length -Heqn in Hne. lia. }
+    rewrite /compile_tp map_length in Hne. lia. }
   inversion Hstep as [|m [tp1 σ1] [tp2 σ2] [tp3 σ3] ? ? Hstep'' Hstep']. subst.
   inversion Hstep'' as [e1' σ1 e2' σ2' efs tpa tpb Htp' Htp2' Hprim].
   injection Htp'. intros -> ->. clear Htp'.
@@ -230,69 +175,38 @@ Proof.
   clear Hstep'' Hprim.
   destruct (decide (length K = 0)) as [HK|HK].
   - apply nil_length_inv in HK as ->. simpl. simpl in *.
-    destruct (is_value e2) eqn:Hval.
-    * destruct (decide (Forall is_value tpa ∧ Forall is_value tpb ∧ Forall is_value efs)) as [[Htp1val [Htp2val Hefsval]]|Hval'].
-      + rewrite compile_tp_app compile_tp_cons !compile_tp_empty // app_nil_l.
-        assert (Hbase' := Hbase). apply base_step_not_value in Hbase' as ->.
-        eapply base_step_in_thread_last_thread with (tid := 0) in Hbase as [tr Htr]; eauto.
-      + apply IH in Hstep' as [tr [tid Htr]]; last first.
-        { rewrite -lt_gt -Nat.neq_0_lt_0. intros Hemp%nil_length_inv.
-          rewrite app_comm_cons !compile_tp_app in Hemp.
-          apply app_eq_nil in Hemp as [Htpa [Htpb Hefs]%app_eq_nil].
-          rewrite compile_tp_cons Hval in Htpb.
-          apply Hval'.
-          split; first by apply compile_tp_empty_inv.
-          split; first by apply compile_tp_empty_inv.
-          by apply compile_tp_empty_inv.
-        }
-        odestruct (base_step_in_thread_completed _ _ _ _ _ _ _ (length (compile_tp tpa)) _ _ Hbase _ _ _) as [tr' [_ Htr']]; eauto; last first.
-        { rewrite compile_tp_app lookup_app_r // Nat.sub_diag compile_tp_cons.
-          assert (Hbase' := Hbase). by apply base_step_not_value in Hbase' as ->. }
-        rewrite compile_tp_app compile_tp_cons.
-        apply base_step_not_value in Hbase as ->.
-        rewrite delete_middle -app_assoc.
-        by rewrite compile_tp_app compile_tp_cons Hval compile_tp_app in Htr.
-      * apply IH in Hstep' as [tr [tid Htr]]; last first.
-        { rewrite -lt_gt -Nat.neq_0_lt_0. intros Hemp%nil_length_inv.
-          rewrite app_comm_cons !compile_tp_app in Hemp.
-          apply app_eq_nil in Hemp as [Htpa [Htpb Hefs]%app_eq_nil].
-          rewrite compile_tp_cons Hval in Htpb.
-          discriminate.
-        }
-        odestruct (base_step_in_thread_not_completed _ _ _ _ _ _ _ (length (compile_tp tpa)) _ _ Hbase _ _ _) as [tr' [_ Htr']]; eauto.
-        1:{ rewrite Hval. eauto. }
-        2:{ rewrite compile_tp_app lookup_app_r // Nat.sub_diag compile_tp_cons.
-          assert (Hbase' := Hbase). by apply base_step_not_value in Hbase' as ->. }
-        rewrite compile_tp_app compile_tp_cons.
-        apply base_step_not_value in Hbase as ->.
-        Search insert length.
-        replace (length (compile_tp tpa)) with (length (compile_tp tpa) + 0) by lia.
-        rewrite insert_app_r /= -app_assoc.
-        by rewrite compile_tp_app compile_tp_cons Hval compile_tp_app in Htr.
-  - apply IH in Hstep' as [tr [tid Htr]]; last first.
-    { rewrite -lt_gt -Nat.neq_0_lt_0. intros Hemp%nil_length_inv.
-      rewrite app_comm_cons !compile_tp_app compile_tp_cons in Hemp.
-      apply app_eq_nil in Hemp as [Htpa [Htpb Hefs]%app_eq_nil].
-      rewrite fill_is_not_value in Htpb; last first. { rewrite -lt_gt -Nat.neq_0_lt_0 //. }
-      discriminate.
+    apply IH in Hstep' as [tr [tid Htr]]; last first.
+    { rewrite /compile_tp map_length app_length /= app_length.
+      rewrite /compile_tp map_length app_length /= in Hne.
+      lia.
     }
-    rewrite compile_tp_app compile_tp_cons fill_is_not_value  in Htr; last first.
-    { rewrite -lt_gt -Nat.neq_0_lt_0 //. }
-    rewrite compile_expr_bind in Htr; last first.
-    { rewrite -lt_gt -Nat.neq_0_lt_0 //. }
-    { admit. }
-    rewrite compile_tp_app compile_tp_cons fill_is_not_value; last first.
-    { rewrite -lt_gt -Nat.neq_0_lt_0 //. }
-    apply step_in_thread with (tp := (compile_tp tpa ++ (v ← compile_expr e1; yield_if_not_val e1;; compile_expr (fill K (Val v));; kill_thread)%itree :: compile_tp tpb)) (tid := length (compile_tp tpa)) (tid' := tid) (k := λ v, (compile_expr (fill K (Val v));; kill_thread)%itree) (tr := tr) in Hbase as [tr' [_ Htr']].
-    * exists tr'. exists (length (compile_tp tpa)).
-      rewrite compile_expr_bind.
-      + rewrite bind_bind. by setoid_rewrite bind_bind.
-      + admit.
-      + rewrite -lt_gt -Nat.neq_0_lt_0 //.
+    apply step_in_thread with (tp := (compile_tp tpa ++ (v ← compile_expr e1; yield_if_not_val e1;; kill_thread)%itree :: compile_tp tpb)) (tid := length (compile_tp tpa)) (tid' := tid) (k := λ v, kill_thread) (tr := tr) in Hbase as [tr' [_ Htr']].
+    * exists tr'. exists (length (compile_tp tpa)). rewrite compile_tp_app //.
     * replace (length (compile_tp tpa)) with (length (compile_tp tpa) + 0) by lia.
       rewrite compile_tp_app in Htr.
       rewrite insert_app_r /= -app_assoc /=.
-      rewrite bind_bind in Htr.
-      by setoid_rewrite bind_bind in Htr.
+      by rewrite /= compile_tp_app in Htr.
+    * rewrite lookup_app_r // Nat.sub_diag //.
+  - apply IH in Hstep' as [tr [tid Htr]]; last first.
+    { rewrite -lt_gt -Nat.neq_0_lt_0. intros Hemp%nil_length_inv.
+      rewrite !compile_tp_app /= in Hemp.
+      apply app_eq_nil in Hemp as [_ [=]].
+    }
+    rewrite compile_tp_app /= compile_tp_app in Htr.
+    rewrite compile_tp_app /=.
+    apply step_in_thread with (tp := (compile_tp tpa ++ (v ← compile_expr e1; yield_if_not_val e1;; compile_expr (fill K (Val v));; trigger EYield;; kill_thread)%itree :: compile_tp tpb)) (tid := length (compile_tp tpa)) (tid' := tid) (k := λ v, (compile_expr (fill K (Val v));; trigger EYield;; kill_thread)%itree) (tr := tr) in Hbase as [tr' [_ Htr']].
+    * exists tr'. exists (length (compile_tp tpa)).
+      rewrite /= compile_expr_bind.
+      + setoid_rewrite fill_not_val; last first. { rewrite -lt_gt -Nat.neq_0_lt_0 //. }
+        rewrite bind_bind. by setoid_rewrite bind_bind.
+      + admit.
+      + rewrite -lt_gt -Nat.neq_0_lt_0 //.
+    * replace (length (compile_tp tpa)) with (length (compile_tp tpa) + 0) by lia.
+      rewrite insert_app_r /= -app_assoc /=.
+      rewrite compile_expr_bind in Htr.
+      + setoid_rewrite fill_not_val in Htr; last first. { rewrite -lt_gt -Nat.neq_0_lt_0 //. }
+        by repeat setoid_rewrite bind_bind in Htr.
+      + admit.
+      + rewrite -lt_gt -Nat.neq_0_lt_0 //.
     * rewrite lookup_app_r // Nat.sub_diag //.
 Admitted.
